Logic/Modal/Standard/Kripke/ModalCompanion.lean
@@ -1,4 +1,5 @@
-import Logic.Propositional.Superintuitionistic
+import Logic.Propositional.Superintuitionistic.Kripke.Semantics
+import Logic.Propositional.Superintuitionistic.Kripke.DP
 import Logic.Modal.Standard.Deduction
 import Logic.Modal.Standard.HilbertStyle
 import Logic.Modal.Standard.Kripke.Semantics
@@ -22,82 +23,82 @@ open System FiniteContext
 open Necessitation
 open LO.Propositional
 
-variable [DecidableEq α] [Inhabited α]
+variable [DecidableEq α] [Inhabited α] [Encodable α]
 
 /-- Gödel Translation -/
-def GTranslation : Superintuitionistic.Formula α → Formula α
+def GoedelTranslation : Superintuitionistic.Formula α → Formula α
   | .atom a  => □(Formula.atom a)
   | .verum   => ⊤
   | .falsum  => ⊥
-  | .and p q => (GTranslation p) ⋏ (GTranslation q)
-  | .or p q  => (GTranslation p) ⋎ (GTranslation q)
-  | .imp p q => □((GTranslation p) ⟶ (GTranslation q))
+  | .and p q => (GoedelTranslation p) ⋏ (GoedelTranslation q)
+  | .or p q  => (GoedelTranslation p) ⋎ (GoedelTranslation q)
+  | .imp p q => □((GoedelTranslation p) ⟶ (GoedelTranslation q))
 
-postfix:75 "ᵍ" => GTranslation
+postfix:75 "ᵍ" => GoedelTranslation
 
-namespace GTranslation
+namespace GoedelTranslation
 
 variable {p q : Superintuitionistic.Formula α}
 
-@[simp] lemma atom_def : (Superintuitionistic.Formula.atom a)ᵍ = □(Formula.atom a) := by simp [GTranslation];
-@[simp] lemma falsum_def : (⊥ : Superintuitionistic.Formula α)ᵍ = ⊥ := by simp [GTranslation];
-@[simp] lemma verum_def : (⊤ : Superintuitionistic.Formula α)ᵍ = ⊤ := by simp [GTranslation];
-@[simp] lemma and_def : (p ⋏ q)ᵍ = pᵍ ⋏ qᵍ := by simp [GTranslation];
-@[simp] lemma or_def : (p ⋎ q)ᵍ = pᵍ ⋎ qᵍ := by simp [GTranslation];
-@[simp] lemma imp_def : (p ⟶ q)ᵍ = □(pᵍ ⟶ qᵍ) := by simp [GTranslation];
-@[simp] lemma neg_def' : (~p)ᵍ = □~(p)ᵍ := by simp [GTranslation, NegDefinition.neg];
+@[simp] lemma atom_def : (Superintuitionistic.Formula.atom a)ᵍ = □(Formula.atom a) := by simp [GoedelTranslation];
+@[simp] lemma falsum_def : (⊥ : Superintuitionistic.Formula α)ᵍ = ⊥ := by simp [GoedelTranslation];
+@[simp] lemma verum_def : (⊤ : Superintuitionistic.Formula α)ᵍ = ⊤ := by simp [GoedelTranslation];
+@[simp] lemma and_def : (p ⋏ q)ᵍ = pᵍ ⋏ qᵍ := by simp [GoedelTranslation];
+@[simp] lemma or_def : (p ⋎ q)ᵍ = pᵍ ⋎ qᵍ := by simp [GoedelTranslation];
+@[simp] lemma imp_def : (p ⟶ q)ᵍ = □(pᵍ ⟶ qᵍ) := by simp [GoedelTranslation];
+@[simp] lemma neg_def' : (~p)ᵍ = □~(p)ᵍ := by simp [GoedelTranslation, NegDefinition.neg];
 
-end GTranslation
+end GoedelTranslation
 
-class ModalCompanion (iΛ : Superintuitionistic.AxiomSet α) (mL : DeductionParameter α) where
-  companion : ∀ {p : Superintuitionistic.Formula α}, iΛ ⊢! p ↔ mL ⊢! pᵍ
+class ModalCompanion (i𝓓 : Superintuitionistic.DeductionParameter α) (m𝓓 : Modal.Standard.DeductionParameter α) where
+  companion : ∀ {p : Superintuitionistic.Formula α}, i𝓓 ⊢! p ↔ m𝓓 ⊢! pᵍ
 
-variable {iΛ : Superintuitionistic.AxiomSet α} {mL : DeductionParameter α}
+variable {i𝓓 : Superintuitionistic.DeductionParameter α} {m𝓓 : DeductionParameter α}
 variable {p q r : Superintuitionistic.Formula α}
 
-lemma axiomTc_GTranslate! [System.K4 mL] : mL ⊢! pᵍ ⟶ □pᵍ := by
+lemma axiomTc_GTranslate! [System.K4 m𝓓] : m𝓓 ⊢! pᵍ ⟶ □pᵍ := by
   induction p using Superintuitionistic.Formula.rec' with
-  | hatom => simp only [GTranslation.atom_def, axiomFour!];
-  | himp => simp only [GTranslation.imp_def, axiomFour!];
-  | hfalsum => simp only [GTranslation.falsum_def, efq!];
+  | hatom => simp only [GoedelTranslation.atom_def, axiomFour!];
+  | himp => simp only [GoedelTranslation.imp_def, axiomFour!];
+  | hfalsum => simp only [GoedelTranslation.falsum_def, efq!];
   | hverum => exact dhyp! (nec! verum!);
   | hand p q ihp ihq =>
-    simp only [GTranslation.and_def];
+    simp only [GoedelTranslation.and_def];
     exact imp_trans! (andReplace! ihp ihq) collect_box_and!
   | hor p q ihp ihq =>
-    simp only [GTranslation.or_def];
+    simp only [GoedelTranslation.or_def];
     exact imp_trans! (disj₃''! (implyOrLeft'! ihp) (implyOrRight'! ihq)) collect_box_or!
 
-instance [System.S4 mL] : System.K4 mL where
+instance [System.S4 m𝓓] : System.K4 m𝓓 where
 
-private lemma provable_efq_of_provable_S4.case_imply₁ [System.K4 mL] : mL ⊢! (p ⟶ q ⟶ p)ᵍ := by
-  simp only [GTranslation.imp_def];
+private lemma provable_efq_of_provable_S4.case_imply₁ [System.K4 m𝓓] : m𝓓 ⊢! (p ⟶ q ⟶ p)ᵍ := by
+  simp only [GoedelTranslation.imp_def];
   exact nec! $ imp_trans! axiomTc_GTranslate! $ axiomK'! $ nec! $ imply₁!;
 
-private lemma provable_efq_of_provable_S4.case_imply₂ [System.S4 mL] : mL ⊢! ((p ⟶ q ⟶ r) ⟶ (p ⟶ q) ⟶ p ⟶ r)ᵍ := by
-  simp only [GTranslation.imp_def];
+private lemma provable_efq_of_provable_S4.case_imply₂ [System.S4 m𝓓] : m𝓓 ⊢! ((p ⟶ q ⟶ r) ⟶ (p ⟶ q) ⟶ p ⟶ r)ᵍ := by
+  simp only [GoedelTranslation.imp_def];
   refine nec! $ imp_trans! (imp_trans! (axiomK'! $ nec! ?b) axiomFour!) $ axiomK'! $ nec! $ imp_trans! (axiomK'! $ nec! imply₂!) axiomK!;
   apply provable_iff_provable.mpr;
   apply deduct_iff.mpr;
   apply deduct_iff.mpr;
-  have : [pᵍ, pᵍ ⟶ □(qᵍ ⟶ rᵍ)] ⊢[mL]! pᵍ := by_axm! (by simp);
-  have : [pᵍ, pᵍ ⟶ □(qᵍ ⟶ rᵍ)] ⊢[mL]! (pᵍ ⟶ □(qᵍ ⟶ rᵍ)) := by_axm! (by simp);
-  have : [pᵍ, pᵍ ⟶ □(qᵍ ⟶ rᵍ)] ⊢[mL]! □(qᵍ ⟶ rᵍ) := (by assumption) ⨀ (by assumption);
+  have : [pᵍ, pᵍ ⟶ □(qᵍ ⟶ rᵍ)] ⊢[m𝓓]! pᵍ := by_axm! (by simp);
+  have : [pᵍ, pᵍ ⟶ □(qᵍ ⟶ rᵍ)] ⊢[m𝓓]! (pᵍ ⟶ □(qᵍ ⟶ rᵍ)) := by_axm! (by simp);
+  have : [pᵍ, pᵍ ⟶ □(qᵍ ⟶ rᵍ)] ⊢[m𝓓]! □(qᵍ ⟶ rᵍ) := (by assumption) ⨀ (by assumption);
   exact axiomT'! this;
 
-private lemma provable_efq_of_provable_S4.case_conj₃ [System.K4 mL] : mL ⊢! (p ⟶ q ⟶ p ⋏ q)ᵍ := by
-  simp only [GTranslation.imp_def, GTranslation.and_def];
+private lemma provable_efq_of_provable_S4.case_conj₃ [System.K4 m𝓓] : m𝓓 ⊢! (p ⟶ q ⟶ p ⋏ q)ᵍ := by
+  simp only [GoedelTranslation.imp_def, GoedelTranslation.and_def];
   exact nec! $ imp_trans! axiomTc_GTranslate! $ axiomK'! $ nec! $ conj₃!
 
-private lemma provable_efq_of_provable_S4.case_disj₃ [System.K4 mL] : mL ⊢! (((p ⟶ r) ⟶ (q ⟶ r) ⟶ (p ⋎ q ⟶ r)))ᵍ := by
-  simp only [GTranslation.imp_def, GTranslation.or_def];
+private lemma provable_efq_of_provable_S4.case_disj₃ [System.K4 m𝓓] : m𝓓 ⊢! (((p ⟶ r) ⟶ (q ⟶ r) ⟶ (p ⋎ q ⟶ r)))ᵍ := by
+  simp only [GoedelTranslation.imp_def, GoedelTranslation.or_def];
   exact nec! $ imp_trans! axiomFour! $ axiomK'! $ nec! $ imp_trans! (axiomK'! $ nec! $ disj₃!) axiomK!;
 
 open provable_efq_of_provable_S4 in
-lemma provable_efq_of_provable_S4 (h : 𝐄𝐅𝐐 ⊢! p) : 𝐒𝟒 ⊢! pᵍ := by
+lemma provable_efq_of_provable_S4 (h : 𝐈𝐧𝐭 ⊢! p) : 𝐒𝟒 ⊢! pᵍ := by
   induction h.some with
   | eaxm ih =>
-    simp_all only [Set.mem_setOf_eq, Superintuitionistic.axiomEFQ];
+    simp_all only [Set.mem_setOf_eq];
     obtain ⟨p, hp⟩ := ih; subst hp;
     exact nec! efq!;
   | mdp hpq hp ihpq ihp =>
@@ -105,67 +106,61 @@ lemma provable_efq_of_provable_S4 (h : 𝐄𝐅𝐐 ⊢! p) : 𝐒𝟒 ⊢! pᵍ
   | verum => apply verum!;
   | imply₁ => exact case_imply₁;
   | imply₂ => exact case_imply₂;
-  | conj₁ => simp only [GTranslation.imp_def, GTranslation.and_def]; exact nec! conj₁!;
-  | conj₂ => simp only [GTranslation.imp_def, GTranslation.and_def]; exact nec! conj₂!;
+  | conj₁ => simp only [GoedelTranslation.imp_def, GoedelTranslation.and_def]; exact nec! conj₁!;
+  | conj₂ => simp only [GoedelTranslation.imp_def, GoedelTranslation.and_def]; exact nec! conj₂!;
   | conj₃ => exact case_conj₃;
-  | disj₁ => simp only [GTranslation.imp_def, GTranslation.or_def]; exact nec! disj₁!;
-  | disj₂ => simp only [GTranslation.imp_def, GTranslation.or_def]; exact nec! disj₂!;
+  | disj₁ => simp only [GoedelTranslation.imp_def, GoedelTranslation.or_def]; exact nec! disj₁!;
+  | disj₂ => simp only [GoedelTranslation.imp_def, GoedelTranslation.or_def]; exact nec! disj₂!;
   | disj₃ => exact case_disj₃;
 
 open Superintuitionistic.Kripke
 open Superintuitionistic.Formula.Kripke
 
-variable [Inhabited (Superintuitionistic.SaturatedConsistentTableau (α := α) 𝐄𝐅𝐐)] --TODO: remove
-
 open Kripke
 
-lemma provable_S4_of_provable_efq : (𝐒𝟒 ⊢! pᵍ) → (𝐄𝐅𝐐 ⊢! p) := by
+lemma provable_S4_of_provable_efq : (𝐒𝟒 ⊢! pᵍ) → (𝐈𝐧𝐭 ⊢! p) := by
   contrapose;
   intro h;
-  obtain ⟨MI, w, h⟩ := by simpa [
-      FrameClass.Intuitionistic,
-      ValidOnFrameClass.iff_models, ValidOnFrameClass,
-      ValidOnModel.iff_models, ValidOnModel
-    ] using not_imp_not.mpr Superintuitionistic.Kripke.complete! h;
+  obtain ⟨iF, _, iV, iV_hereditary, w, h⟩ := by simpa [ValidOnFrameClass, ValidOnFrame, ValidOnModel] using not_imp_not.mpr Superintuitionistic.Kripke.complete! h;
 
-  have MTrans := MI.frame_prop.1;
-  have MRefl := MI.frame_prop.2;
-
-  let M : Modal.Standard.Kripke.Model α := { Frame := { Rel := MI.frame }, Valuation := MI.valuation};
-  have h₁ : ∀ q (v : Superintuitionistic.SaturatedConsistentTableau (α := α) 𝐄𝐅𝐐), (MI, v) ⊧ q ↔ (Modal.Standard.Formula.Kripke.Satisfies M v (qᵍ)) := by
+  let M : Modal.Standard.Kripke.Model α := { Frame := { Rel := iF.Rel }, Valuation := iV };
+  have h₁ : ∀ q v, Satisfies ⟨iF, iV, iV_hereditary⟩ v q ↔ (Modal.Standard.Formula.Kripke.Satisfies M v (qᵍ)) := by
     intro q v;
     induction q using Superintuitionistic.Formula.rec' generalizing v with
     | hatom a =>
       constructor;
       . intro _ _ h;
         simp_all only [Satisfies.iff_models, Satisfies, Formula.Kripke.Satisfies];
-        exact MI.hereditary h a (by assumption);
+        exact iV_hereditary h (by assumption);
       . intro h;
-        simpa only [Satisfies.iff_models, Satisfies, Formula.Kripke.Satisfies] using h v (MRefl v);
+        simpa only [Satisfies.iff_models, Satisfies, Formula.Kripke.Satisfies] using h v $ iF.Rel_refl v;
     | _ => simp_all;
   have : ¬(Modal.Standard.Formula.Kripke.Satisfies M w (pᵍ)) := (h₁ p w).not.mp h;
 
-  by_contra hC;
-  have := by simpa using Modal.Standard.Kripke.sound!_on_frameclass hC;
-  have : (Modal.Standard.Formula.Kripke.Satisfies M w (pᵍ)) := this M.Frame (
-      iff_definability_memAxiomSetFrameClass
+  apply not_imp_not.mpr $ Modal.Standard.Kripke.sound!_on_frameclass;
+  simp [Formula.Kripke.ValidOnFrame, Formula.Kripke.ValidOnModel];
+  existsi M.Frame;
+  constructor;
+  . apply Modal.Standard.Kripke.iff_definability_memAxiomSetFrameClass
       (show Kripke.Definability _ (λ F => Reflexive F.Rel ∧ Transitive F.Rel) by simpa using instGeachDefinability (L := 𝐒𝟒))
-      |>.mpr ⟨MRefl, MTrans⟩
-    ) M.Valuation w;
-  contradiction;
+      |>.mpr;
+    constructor;
+    . exact iF.Rel_refl;
+    . exact iF.Rel_trans;
+  . use M.Valuation, w;
 
 /-- a.k.a. _Gödel-McKinsey-Tarski Theorem_ -/
-theorem provable_efq_iff_provable_S4 : 𝐄𝐅𝐐 ⊢! p ↔ 𝐒𝟒 ⊢! pᵍ := ⟨provable_efq_of_provable_S4, provable_S4_of_provable_efq⟩
-instance : ModalCompanion (α := α) 𝐄𝐅𝐐 𝐒𝟒 := ⟨provable_efq_iff_provable_S4⟩
+theorem provable_efq_iff_provable_S4 : 𝐈𝐧𝐭 ⊢! p ↔ 𝐒𝟒 ⊢! pᵍ := ⟨provable_efq_of_provable_S4, provable_S4_of_provable_efq⟩
+instance : ModalCompanion (α := α) 𝐈𝐧𝐭 𝐒𝟒 := ⟨provable_efq_iff_provable_S4⟩
 
 
-lemma dp_of_mdp [ModalDisjunctive mL] [ModalCompanion iΛ mL] [S4 mL] : iΛ ⊢! p ⋎ q → iΛ ⊢! p ∨ iΛ ⊢! q := by
+lemma dp_of_mdp [ModalDisjunctive m𝓓] [ModalCompanion i𝓓 m𝓓] [S4 m𝓓] : i𝓓 ⊢! p ⋎ q → i𝓓 ⊢! p ∨ i𝓓 ⊢! q := by
     intro hpq;
-    have : mL ⊢! □pᵍ ⋎ □qᵍ := disj₃'! (implyOrLeft'! axiomTc_GTranslate!) (implyOrRight'! axiomTc_GTranslate!) (by simpa using ModalCompanion.companion.mp hpq);
+    have : m𝓓 ⊢! □pᵍ ⋎ □qᵍ := disj₃'! (implyOrLeft'! axiomTc_GTranslate!) (implyOrRight'! axiomTc_GTranslate!) (by simpa using ModalCompanion.companion.mp hpq);
     cases ModalDisjunctive.modal_disjunctive this with
     | inl h => left; exact ModalCompanion.companion.mpr h;
     | inr h => right; exact ModalCompanion.companion.mpr h;
 
-theorem disjunctive_of_modalDisjunctive [ModalDisjunctive mL] [ModalCompanion iΛ mL] [S4 mL] : Disjunctive iΛ := ⟨dp_of_mdp (iΛ := iΛ) (mL := mL)⟩
+theorem disjunctive_of_modalDisjunctive [ModalDisjunctive m𝓓] [ModalCompanion i𝓓 m𝓓] [S4 m𝓓] : Disjunctive i𝓓 := ⟨dp_of_mdp (i𝓓 := i𝓓) (m𝓓 := m𝓓)⟩
 
 end LO.Modal.Standard
