Logic/Propositional/Superintuitionistic/Kripke/DP.lean
@@ -19,106 +19,115 @@ open Formula Formula.Kripke
 
 namespace Kripke
 
-variable {α} [DecidableEq α]
+variable {α} [Inhabited α] [DecidableEq α] [Encodable α]
 variable {p q : Formula α}
 
-def IntDPCounterexampleModel (M₁ : Model (𝐈𝐧𝐭 W₁ α)) (M₂ : Model (𝐈𝐧𝐭 W₂ α)) (w₁ : W₁) (w₂ : W₂) : Model (𝐈𝐧𝐭 (Unit ⊕ W₁ ⊕ W₂) α) where
-  frame w v :=
+abbrev IntDPCounterexampleFrame (F₁ : Frame.{u}) (F₂ : Frame.{u}) (w₁ : F₁.World) (w₂ : F₂.World) : Frame where
+  World := Unit ⊕ F₁.World ⊕ F₂.World;
+  Rel w v :=
     match w, v with
     | (Sum.inl _), (Sum.inl _) => True
-    | (Sum.inl _), (Sum.inr $ Sum.inl v) => M₁.frame w₁ v
-    | (Sum.inl _), (Sum.inr $ Sum.inr v) => M₂.frame w₂ v
-    | (Sum.inr $ Sum.inl w), (Sum.inr $ Sum.inl v) => M₁.frame w v
-    | (Sum.inr $ Sum.inr w), (Sum.inr $ Sum.inr v) => M₂.frame w v
+    | (Sum.inl _), (Sum.inr $ Sum.inl v) => w₁ ≺ v
+    | (Sum.inl _), (Sum.inr $ Sum.inr v) => w₂ ≺ v
+    | (Sum.inr $ Sum.inl w), (Sum.inr $ Sum.inl v) => w ≺ v
+    | (Sum.inr $ Sum.inr w), (Sum.inr $ Sum.inr v) => w ≺ v
     | _, _ => False
-  valuation w a :=
+  Rel_refl := by
+    simp only [Reflexive, Sum.forall, forall_const, true_and];
+    constructor;
+    . exact F₁.Rel_refl;
+    . exact F₂.Rel_refl;
+  Rel_trans := by
+    simp only [Transitive, Sum.forall, forall_true_left, imp_self, forall_const, true_and, IsEmpty.forall_iff, implies_true, and_true, and_self, imp_false];
+    constructor;
+    . constructor;
+      . intro _ _; apply F₁.Rel_trans;
+      . intro _ _; apply F₂.Rel_trans;
+    . constructor;
+      . intro _ _; apply F₁.Rel_trans;
+      . intro _ _; apply F₂.Rel_trans;
+  Rel_antisymm := by
+    simp only [Antisymmetric, Sum.forall, forall_true_left, forall_const, IsEmpty.forall_iff, implies_true, and_self, imp_false, Sum.inr.injEq, true_and, Sum.inl.injEq, and_true];
+    constructor;
+    . exact F₁.Rel_antisymm;
+    . exact F₂.Rel_antisymm;
+
+abbrev IntDPCounterexampleModel (M₁ : Model α) (M₂ : Model α) (w₁ : M₁.World) (w₂ : M₂.World) : Model α where
+  Frame := IntDPCounterexampleFrame M₁.Frame M₂.Frame w₁ w₂;
+  Valuation w a :=
     match w with
-    | Sum.inr $ Sum.inl w => M₁.valuation w a
-    | Sum.inr $ Sum.inr w => M₂.valuation w a
+    | Sum.inr $ Sum.inl w => M₁.Valuation w a
+    | Sum.inr $ Sum.inr w => M₂.Valuation w a
     | _ => False
   hereditary := by
-    simp only [Sum.forall, imp_false, not_false_eq_true, implies_true, forall_true_left, forall_const, IsEmpty.forall_iff, and_self, true_and, and_true];
+    simp only [Sum.forall, imp_false, not_false_eq_true, implies_true, forall_true_left, forall_const, IsEmpty.forall_iff, and_self, and_true, true_and];
     constructor;
     . intro _ _; apply M₁.hereditary;
     . intro _ _; apply M₂.hereditary;
-  frame_prop := by
-    constructor;
-    . simp only [Transitive, Sum.forall, forall_true_left, imp_self, forall_const, true_and, IsEmpty.forall_iff, implies_true, and_true, and_self, imp_false];
-      constructor;
-      . constructor;
-        . intro _ _; apply M₁.frame_prop.1;
-        . intro _ _; apply M₂.frame_prop.1;
-      . constructor;
-        . intro _ _; apply M₁.frame_prop.1;
-        . intro _ _; apply M₂.frame_prop.1;
-    . simp only [Reflexive, Sum.forall, forall_const, true_and];
-      constructor;
-      . intros; apply M₁.frame_prop.2;
-      . intros; apply M₂.frame_prop.2;
 
-variable {M₁ : Model (𝐈𝐧𝐭 W₁ α)} {M₂ : Model (𝐈𝐧𝐭 W₂ α)}
+variable {M₁ : Model α} {M₂ : Model α}
 
-lemma satisfies_left_on_IntDPCounterexampleModel : ((M₁, w) ⊧ p) ↔ ((IntDPCounterexampleModel M₁ M₂ w₁ w₂, (Sum.inr $ Sum.inl w : (Unit ⊕ W₁ ⊕ W₂))) ⊧ p) := by
+lemma satisfies_left_on_IntDPCounterexampleModel :
+  (Satisfies M₁ w p) ↔ (Satisfies (IntDPCounterexampleModel M₁ M₂ w₁ w₂) (Sum.inr $ Sum.inl w) p) := by
+  -- ((M₁, w) ⊧ p) ↔ ((IntDPCounterexampleModel M₁ M₂ w₁ w₂, (Sum.inr $ Sum.inl w : (Unit ⊕ W₁ ⊕ W₂))) ⊧ p) := by
   induction p using rec' generalizing w with
   | himp p q ihp ihq =>
     constructor;
     . simp only [Satisfies.imp_def];
-      intro h v hv hp;
-      replace ⟨v, hv, hv'⟩ : ∃ v', M₁.frame w v' ∧ v = (Sum.inr (Sum.inl v')) := by
-        simp [IntDPCounterexampleModel] at hv;
-        split at hv;
+      intro h X hWX hp;
+      obtain ⟨x, hx, ex⟩ : ∃ x, w ≺ x ∧ (Sum.inr $ Sum.inl x) = X := by
+        replace hWX : (IntDPCounterexampleModel M₁ M₂ w₁ w₂).Frame.Rel _ X := hWX;
+        simp [IntDPCounterexampleFrame] at hWX;
+        split at hWX;
         all_goals simp_all;
-      subst hv';
-      exact ihq.mp $ h hv $ ihp.mpr hp;
+      subst ex;
+      exact ihq.mp $ h hx $ ihp.mpr hp;
     . simp only [Satisfies.imp_def];
       intro h v hv hp;
       exact ihq.mpr $ h (by simpa [IntDPCounterexampleModel]) $ ihp.mp hp;
   | _ => simp_all [IntDPCounterexampleModel, Satisfies.iff_models, Satisfies];
 
-lemma satisfies_right_on_IntDPCounterexampleModel : ((M₂, w) ⊧ p) ↔ ((IntDPCounterexampleModel M₁ M₂ w₁ w₂, (Sum.inr $ Sum.inr w : (Unit ⊕ W₁ ⊕ W₂))) ⊧ p) := by
+lemma satisfies_right_on_IntDPCounterexampleModel :
+  (Satisfies M₂ w p) ↔ (Satisfies (IntDPCounterexampleModel M₁ M₂ w₁ w₂) (Sum.inr $ Sum.inr w) p) := by
+  -- : ((M₂, w) ⊧ p) ↔ ((IntDPCounterexampleModel M₁ M₂ w₁ w₂, (Sum.inr $ Sum.inr w : (Unit ⊕ W₁ ⊕ W₂))) ⊧ p) := by
   induction p using rec' generalizing w with
   | himp p q ihp ihq =>
     constructor;
     . simp only [Satisfies.imp_def];
-      intro h v hv hp;
-      replace ⟨v, hv, hv'⟩ : ∃ v', M₂.frame w v' ∧ v = (Sum.inr (Sum.inr v')) := by
-        simp [IntDPCounterexampleModel] at hv;
-        split at hv;
+      intro h X hWX hp;
+      obtain ⟨x, hx, ex⟩ : ∃ x, w ≺ x ∧ (Sum.inr $ Sum.inr x) = X := by
+        replace hWX : (IntDPCounterexampleModel M₁ M₂ w₁ w₂).Frame.Rel _ X := hWX;
+        simp [IntDPCounterexampleFrame] at hWX;
+        split at hWX;
         all_goals simp_all;
-      subst hv';
-      exact ihq.mp $ h hv $ ihp.mpr hp;
+      subst ex;
+      exact ihq.mp $ h hx $ ihp.mpr hp;
     . simp only [Satisfies.imp_def];
       intro h v hv hp;
       exact ihq.mpr $ h (by simpa [IntDPCounterexampleModel]) $ ihp.mp hp;
   | _ => simp_all [IntDPCounterexampleModel, Satisfies.iff_models, Satisfies];
 
-
-theorem disjunctive_int : 𝐄𝐅𝐐 ⊢! p ⋎ q → (𝐄𝐅𝐐 ⊢! p ∨ 𝐄𝐅𝐐 ⊢! q) := by
+theorem disjunctive_int : 𝐈𝐧𝐭 ⊢! p ⋎ q → 𝐈𝐧𝐭 ⊢! p ∨ 𝐈𝐧𝐭 ⊢! q := by
   contrapose;
-  intro hC; simp [not_or] at hC;
+  intro hC; push_neg at hC;
   have ⟨hnp, hnq⟩ := hC;
-  obtain ⟨Mp, wp, hp⟩ := by simpa [ValidOnFrameClass.iff_models, ValidOnFrameClass, ValidOnModel.iff_models, ValidOnModel] using (not_imp_not.mpr complete!) hnp;
-  obtain ⟨Mq, wq, hq⟩ := by simpa [ValidOnFrameClass.iff_models, ValidOnFrameClass, ValidOnModel.iff_models, ValidOnModel] using (not_imp_not.mpr complete!) hnq;
+  obtain ⟨Fp, _, Vp, hVp, wp, hp⟩ := by simpa [ValidOnFrameClass, ValidOnFrame, ValidOnModel] using not_imp_not.mpr complete! hnp;
+  obtain ⟨Fq, _, Vq, hVq, wq, hq⟩ := by simpa [ValidOnFrameClass, ValidOnFrame, ValidOnModel] using not_imp_not.mpr complete! hnq;
   apply (not_imp_not.mpr sound!);
-  simp [ValidOnFrameClass.iff_models, ValidOnFrameClass, ValidOnModel.iff_models, ValidOnModel];
 
-  let M := IntDPCounterexampleModel Mp Mq wp wq;
-  existsi M, Sum.inl ();
+  simp [ValidOnFrameClass, ValidOnFrame, ValidOnModel];
+  let M : Model α := IntDPCounterexampleModel ⟨Fp, Vp, hVp⟩ ⟨Fq, Vq, hVq⟩ wp wq;
+  existsi M.Frame;
+  constructor;
+  . apply iff_definability_memAxiomSetFrameClass AxiomSet.EFQ.definability |>.mpr;
+    trivial;
+  . existsi M.Valuation, M.hereditary, Sum.inl ();
+    push_neg;
+    constructor;
+    . exact not_imp_not.mpr (Satisfies.formula_hereditary (by apply Fp.Rel_refl)) $ satisfies_left_on_IntDPCounterexampleModel.not.mp hp;
+    . exact not_imp_not.mpr (Satisfies.formula_hereditary (by apply Fq.Rel_refl)) $ satisfies_right_on_IntDPCounterexampleModel.not.mp hq;
 
-  have hup : M.frame (Sum.inl ()) (Sum.inr $ Sum.inl wp) := by
-    simp [M, IntDPCounterexampleModel];
-    apply Mp.frame_prop.2;
-
-  have huq : M.frame (Sum.inl ()) (Sum.inr $ Sum.inr wq) := by
-    simp [M, IntDPCounterexampleModel];
-    apply Mq.frame_prop.2;
-
-  have : ¬(M, Sum.inl ()) ⊧ p := not_imp_not.mpr (Satisfies.hereditary (by simp_all [FrameClass.Intuitionistic]) hup) $ satisfies_left_on_IntDPCounterexampleModel.not.mp hp;
-  have : ¬(M, Sum.inl ()) ⊧ q := not_imp_not.mpr (Satisfies.hereditary (by simp_all [FrameClass.Intuitionistic]) huq) $ satisfies_right_on_IntDPCounterexampleModel.not.mp hq;
-
-  simp_all;
-
-instance : Disjunctive (𝐄𝐅𝐐 : AxiomSet α) := ⟨disjunctive_int⟩
+instance : Disjunctive (𝐈𝐧𝐭 : DeductionParameter α) := ⟨disjunctive_int⟩
 
 end Kripke
 
