Logic/Vorspiel/BinaryRelations.lean
@@ -7,7 +7,8 @@ section
 variable {α : Type u} (rel : α → α → Prop)
 local infix:50 " ≺ " => rel
 
-def Euclidean := ∀ ⦃w₁ w₂ w₃⦄, w₁ ≺ w₂ → w₁ ≺ w₃ → (w₂ ≺ w₃)
+-- NOTE: `w₁ ≺ w₂ → w₁ ≺ w₃ → w₂ ≺ w₃`とする流儀もある
+def Euclidean := ∀ ⦃w₁ w₂ w₃⦄, w₁ ≺ w₂ → w₁ ≺ w₃ → w₃ ≺ w₂
 
 def Serial := ∀ w₁, ∃ w₂, w₁ ≺ w₂
 
@@ -20,6 +21,8 @@ def Functional := ∀ ⦃w₁ w₂ w₃⦄, w₁ ≺ w₂ ∧ w₁ ≺ w₃ → 
 def RightConvergent := ∀ ⦃w₁ w₂ w₃⦄, w₁ ≺ w₂ ∧ w₁ ≺ w₃ → w₂ ≺ w₃ ∨ w₃ ≺ w₂ ∨ w₂ = w₃
 
 def Extensive := ∀ ⦃x y⦄, x ≺ y → x = y
+
+def Antisymmetric := ∀ ⦃w₁ w₂⦄, w₁ ≺ w₂ → w₂ ≺ w₁ → w₁ = w₂
 
 abbrev ConverseWellFounded := WellFounded $ flip (· ≺ ·)
 
@@ -45,17 +48,17 @@ lemma serial_of_refl : Serial rel := by
 lemma eucl_of_symm_trans : Euclidean rel := by
   intro w₁ w₂ w₃ r₁₂ r₁₃;
   have r₂₁ := hSymm r₁₂;
-  exact hTrans r₂₁ r₁₃;
+  exact hSymm $ hTrans r₂₁ r₁₃;
 
 -- B + 5 → 4
 lemma trans_of_symm_eucl : Transitive rel := by
   rintro w₁ w₂ w₃ r₁₂ r₂₃;
-  exact hEucl (hSymm r₁₂) r₂₃;
+  exact hSymm $ hEucl (hSymm r₁₂) r₂₃;
 
 -- T + 5 → B
 lemma symm_of_refl_eucl : Symmetric rel := by
   intro w₁ w₂ r₁₂;
-  exact hEucl r₁₂ (hRefl w₁);
+  exact hEucl (hRefl w₁) r₁₂;
 
 -- T + 5 → 4
 lemma trans_of_refl_eucl : Transitive rel := by
